src/impl/TLS13.Impl.Serializer.Certificate.fsti
@@ -1,0 +1,37 @@
+module TLS13.Impl.Serializer.Certificate
+
+#lang-pulse
+
+open Pulse.Lib.Pervasives
+open Pulse.Lib.Array.PtsTo
+
+module B = TLS13.Bytes
+module L = TLS13.Impl.Messages
+module M = TLS13.Messages
+module Seq = FStar.Seq
+module SZ = FStar.SizeT
+module U8 = FStar.UInt8
+module WS = TLS13.Wire.Spec
+
+fn serialize_certificate_from_credential
+  (#cert: erased M.certificate_msg)
+  (lcert: L.certificate_msg)
+  (out: array U8.t)
+  (out_len: SZ.t)
+  (#old_bytes: erased B.bytes)
+  requires L.is_valid_certificate_msg lcert (Ghost.reveal cert) **
+           pts_to out (Ghost.reveal old_bytes) **
+           pure (B.length (Ghost.reveal old_bytes) == SZ.v out_len /\
+                 lcert.L.certificate_msg_cert_count == 1sz /\
+                 (exists (certificate:B.bytes).
+                   (Ghost.reveal cert).M.chain == [certificate]) /\
+                 SZ.v out_len ==
+                   B.length (WS.serialize_certificate_from_credential (Ghost.reveal cert)))
+  returns written: (n:SZ.t{SZ.v n <= SZ.v out_len})
+  ensures exists* out_bytes.
+          L.is_valid_certificate_msg lcert (Ghost.reveal cert) **
+          pts_to out out_bytes **
+          pure (B.length out_bytes == SZ.v out_len /\
+                SZ.v written == SZ.v out_len /\
+                Seq.equal out_bytes
+                  (WS.serialize_certificate_from_credential (Ghost.reveal cert)))
