src/impl/TLS13.Impl.Serializer.Finished.fsti
@@ -1,0 +1,37 @@
+module TLS13.Impl.Serializer.Finished
+
+#lang-pulse
+
+open Pulse.Lib.Pervasives
+open Pulse.Lib.Array.PtsTo
+
+module B = TLS13.Bytes
+module L = TLS13.Impl.Messages
+module M = TLS13.Messages
+module Seq = FStar.Seq
+module SZ = FStar.SizeT
+module T = TLS13.Types
+module U8 = FStar.UInt8
+module V = Pulse.Lib.Vec
+module WS = TLS13.Wire.Spec
+
+fn serialize_server_finished
+  (#fin: erased M.finished)
+  (lfin: L.finished)
+  (out: array U8.t)
+  (out_len: SZ.t)
+  (#old_bytes: erased B.bytes)
+  requires L.is_valid_finished lfin (Ghost.reveal fin) **
+           pts_to out (Ghost.reveal old_bytes) **
+           pure (B.length (Ghost.reveal old_bytes) == SZ.v out_len /\
+                 SZ.v out_len == 36)
+  returns written: (n:SZ.t{SZ.v n <= SZ.v out_len})
+  ensures exists* out_bytes.
+          L.is_valid_finished lfin (Ghost.reveal fin) **
+          pts_to out out_bytes **
+          pure (B.length out_bytes == 36 /\
+                SZ.v written == 36 /\
+                Seq.equal out_bytes
+                  (WS.serialize_server_finished (Ghost.reveal fin)) /\
+                WS.parse_tls_message T.Handshake out_bytes ==
+                  Some (M.TlsHandshake (M.Finished (Ghost.reveal fin))))
