src/impl/TLS13.Impl.Serializer.ServerHello.fsti
@@ -1,0 +1,62 @@
+module TLS13.Impl.Serializer.ServerHello
+
+#lang-pulse
+
+open Pulse.Lib.Pervasives
+open Pulse.Lib.Array.PtsTo
+
+module B = TLS13.Bytes
+module CS = TLS13.Spec.ConnectionState
+module L = TLS13.Impl.Messages
+module M = TLS13.Messages
+module Seq = FStar.Seq
+module SZ = FStar.SizeT
+module T = TLS13.Types
+module U8 = FStar.UInt8
+module WS = TLS13.Wire.Spec
+
+fn serialize_server_hello_from_selection
+  (#sh: erased M.server_hello)
+  (lsh: L.server_hello)
+  (out: array U8.t)
+  (out_len: SZ.t)
+  (#old_bytes: erased B.bytes)
+  requires L.is_valid_server_hello lsh (Ghost.reveal sh) **
+           pts_to out (Ghost.reveal old_bytes) **
+           pure (B.length (Ghost.reveal old_bytes) == SZ.v out_len /\
+                 SZ.v out_len == 90)
+  returns written: (n:SZ.t{SZ.v n <= SZ.v out_len})
+  ensures exists* out_bytes.
+          L.is_valid_server_hello lsh (Ghost.reveal sh) **
+          pts_to out out_bytes **
+          pure (B.length out_bytes == 90 /\
+                SZ.v written == 90 /\
+                Seq.equal out_bytes
+                  (WS.serialize_server_hello_from_selection (Ghost.reveal sh)))
+
+fn serialize_server_hello_record_from_selection
+  (#sh: erased M.server_hello)
+  (lsh: L.server_hello)
+  (out: array U8.t)
+  (out_len: SZ.t)
+  (#old_bytes: erased B.bytes)
+  requires L.is_valid_server_hello lsh (Ghost.reveal sh) **
+           pts_to out (Ghost.reveal old_bytes) **
+           pure (B.length (Ghost.reveal old_bytes) == SZ.v out_len /\
+                 SZ.v out_len == 95)
+  returns written: (n:SZ.t{SZ.v n <= SZ.v out_len})
+  ensures exists* out_bytes.
+          L.is_valid_server_hello lsh (Ghost.reveal sh) **
+          pts_to out out_bytes **
+          pure (B.length out_bytes == 95 /\
+                SZ.v written == 95 /\
+                Seq.equal out_bytes
+                  (WS.serialize_record
+                    T.Handshake
+                    (WS.serialize_server_hello_from_selection (Ghost.reveal sh))) /\
+                WS.parse_record out_bytes ==
+                  Some
+                    (T.Handshake,
+                     WS.serialize_server_hello_from_selection (Ghost.reveal sh),
+                     95) /\
+                CS.raw_records_exactly out_bytes T.Handshake 1)
